Intuition failed

src/PlutusIR/Semantics/Static/NoDup'_prototype_normalise.v
@@ -1,5 +1,6 @@
 From Coq Require Import Lists.List.
 From Coq Require Import Strings.String.
+From Coq Require Import micromega.Lia.
 
 From PlutusCert Require Import Util.List util.
 
@@ -19,6 +20,12 @@ Qed.
 Inductive kind :=
   | Kind_Base : kind
   | Kind_Arrow : kind -> kind -> kind.
+
+Fixpoint kind_size (k : kind) : nat :=
+  match k with
+  | Kind_Base => 1
+  | Kind_Arrow K1 K2 => (kind_size K1) + (kind_size K2)
+  end.
 
 (** Types *)
 Inductive ty :=
@@ -142,65 +149,86 @@ Definition P_ND (X : string) (T : ty) (Δ : list (string * ty)) :=
 Definition P_ND2 (Δ1 Δ2 : list (string * ty)) :=
     forall X T T', lookup X Δ1 = Some T -> lookup X Δ2 = Some T' -> T <> T' -> False.
 
-Definition P_ND2' (Δ1 Δ2 : list (string * ty)) :=
-    forall X T T', In (X, T) Δ1 -> In (X, T') Δ2 -> T = T'.
+Definition P_ND2' (Δ1 Δ2 : list (string * (kind * ty))) :=
+    forall X KT KT', In (X, KT) Δ1 -> In (X, KT') Δ2 -> KT = KT'.
 
 (* If a binder occurs multiple times, and we started with a GU term,
     we must have had a beta reduction. This we only do with normal types.
 *)
-Definition P_Dup_Normal (Δ1 Δ2 : list (string * ty)) :=
-    forall X T T', In (X, T) Δ1 -> In (X, T') Δ2 -> T = T' -> normal_Ty T.
+Definition P_Dup_Normal (Δ1 Δ2 : list (string * (kind * ty))) :=
+    forall X T T' K1 K2, In (X, (K1, T)) Δ1 -> In (X, (K2, T')) Δ2 -> (K1, T) = (K2, T') -> normal_Ty T.
 
-Definition P_BF (Δ : list (string * ty)) (Γ : list string) :=
+Definition P_BF (Δ : list (string * (kind *ty))) (Γ : list string) :=
     forall X, In X Γ -> ~ In X (map fst Δ).
+
+
+(** Kinding of types *)
+Reserved Notation "Δ '|-*' T ':' K" (at level 40, T at level 0, K at level 0).
+Inductive has_kind : list (string * kind) -> ty -> kind -> Prop :=
+  | K_Var : forall Δ X K,
+      lookup X Δ = Some K ->
+      Δ |-* (Ty_Var X) : K
+  | K_Lam : forall Δ X K1 T K2,
+      ((X, K1) :: Δ) |-* T : K2 ->
+      Δ |-* (Ty_Lam X K1 T) : (Kind_Arrow K1 K2)
+  | K_App : forall Δ T1 T2 K1 K2,
+      Δ |-* T1 : (Kind_Arrow K1 K2) ->
+      (drop_btv Δ (btv T1)) |-* T2 : K1 -> (* This rule makes that a well-kinded type can never have capture when evaluated one step*)
+      Δ |-* (Ty_App T1 T2) : K2
+where "Δ '|-*' T ':' K" := (has_kind Δ T K).
 
 (*
     Δ keeps track of lambda bodies, to make sure we never have dissimilar bodies for the same binder
     Γ keeps track of ftvs: no ftv may be bound somewhere else
 *)
-Reserved Notation "Δ : Γ '⊢' T" (at level 40, Γ at level 0, T at level 0, no associativity).
-Inductive WK_Dup' : list (string * ty) -> list string -> ty -> Prop :=
-  | ND_Var : forall Γ X,
+Reserved Notation "Ξ ,, Δ : Γ '⊢' T # K" (at level 40, Δ at level 0, Γ at level 0, T at level 0, no associativity).
+Inductive WK : list (string * kind) -> list (string * (kind * ty)) -> list string -> ty -> kind -> Prop :=
+  | ND_Var : forall Γ X Ξ K,
       In X Γ ->
-      [] : Γ ⊢ (Ty_Var X)   (* I changed this to nil, so that we cannot have random stuff in there*)
-  | ND_Lam : forall Δ Γ X K1 T,
-      Δ : (X::Γ) ⊢ T ->
-      (* P_ND X T Δ ->  *)
-      (* Do we need this? *)
-      P_BF ((X, T)::Δ) Γ -> (* uhm *)
-      ((X, T)::Δ) : Γ ⊢ (Ty_Lam X K1 T)
-  | ND_App : forall Δ1 Δ2 Γ T1 T2 ,
-      Δ1 : Γ ⊢ T1 ->
-      Δ2 : Γ ⊢ T2 ->
+      lookup X Ξ = Some K ->
+      Ξ ,, [] : Γ ⊢ (Ty_Var X) # K   (* I changed this to nil, so that we cannot have random stuff in there*)
+  | ND_Lam : forall Δ Γ X K1 T Ξ K2,
+      ((X, K1)::Ξ) ,, Δ : (X::Γ) ⊢ T # K2 ->
+      P_BF ((X, (K1, T))::Δ) Γ -> 
+
+      Ξ ,, ((X, (K1, T))::Δ) : Γ ⊢ (Ty_Lam X K1 T) # (Kind_Arrow K1 K2)
+  | ND_App : forall Δ1 Δ2 Γ T1 T2 Ξ K1 K2,
+      Ξ ,, Δ1 : Γ ⊢ T1 # (Kind_Arrow K1 K2) ->
+      Ξ ,, Δ2 : Γ ⊢ T2 # K1 ->
       P_ND2' Δ1 Δ2 ->
       P_Dup_Normal Δ1 Δ2 ->
       P_BF (Δ1 ++ Δ2) Γ ->
-      (Δ1 ++ Δ2) : Γ ⊢ (Ty_App T1 T2)
-where "Δ : Γ '⊢' T" := (WK_Dup' Δ Γ T).
+      Ξ ,, (Δ1 ++ Δ2) : Γ ⊢ (Ty_App T1 T2) # K2
+where "Ξ ,, Δ : Γ '⊢' T # K" := (WK Ξ Δ Γ T K).
 
 
 Create HintDb noDup_db.
-Hint Constructors WK_Dup' : noDup_db.
+Hint Constructors WK : noDup_db.
 
 Definition KB := Kind_Base.
+
+Lemma P_ND2'_sym Δ1 Δ2 :
+  P_ND2' Δ1 Δ2 ->
+  P_ND2' Δ2 Δ1.
+Admitted.
 
 (* 
 (λX. λY. X Y)   (ΛY. Y)
 *)
 Definition t1_bad := Ty_App
-        ( Ty_Lam "X" KB (Ty_Lam "Y" KB (Ty_App (Ty_Var "X") (Ty_Var "Y"))))
+        ( Ty_Lam "X" (Kind_Arrow KB KB) (Ty_Lam "Y" KB (Ty_App (Ty_Var "X") (Ty_Var "Y"))))
         (Ty_Lam "Y" KB (Ty_Var "Y")).
 
 Lemma t1_bad__not_wk :
-    forall Δ Γ,
-        (Δ : Γ ⊢ t1_bad) -> False.
+    forall Ξ Δ Γ K,
+        (Ξ ,, Δ : Γ ⊢ t1_bad # K ) -> False.
 Proof.
     intros.
     unfold t1_bad in H.
     inversion H; subst; clear H.
     inversion H3; subst; clear H3.
     inversion H2; subst; clear H2.
-    inversion H5; subst; clear H5.
+    inversion H6; subst; clear H6.
     unfold P_ND2' in H4.
     specialize H4 with (X := "Y") (T := Ty_App (Ty_Var "X") (Ty_Var "Y"))
                 (T' := (Ty_Var "Y")).
@@ -217,8 +245,8 @@ Definition t2_bad := Ty_App
         (Ty_Lam "X" KB (Ty_Lam "Y" KB (Ty_App (Ty_Var "X") (Ty_Var "Y")))).
 
 Lemma t2_bad__not_wk :
-    forall Δ Γ,
-        (Δ : Γ ⊢ t2_bad) -> False.
+    forall Ξ Δ Γ K,
+        (Ξ ,, Δ : Γ ⊢ t2_bad # K) -> False.
 Proof.
     intros.
     unfold t2_bad in H.
@@ -235,51 +263,69 @@ Proof.
 Qed.
 
 Definition t2_good := Ty_App
-        (Ty_Lam "X" KB (Ty_App (Ty_Lam "Y" KB (Ty_App (Ty_Var "Y") (Ty_Var "X"))) (Ty_Lam "Z" KB (Ty_Var "X"))))
+        (Ty_Lam "X" ((Kind_Arrow KB KB))
+          (Ty_App (Ty_Lam "Y" (Kind_Arrow (Kind_Arrow KB KB) (Kind_Arrow KB KB)) (Ty_App (Ty_Var "Y") (Ty_Var "X"))) 
+                  (Ty_Lam "Z" (Kind_Arrow KB KB) (Ty_Var "X"))))
         (Ty_Lam "V" KB (Ty_Var "V")).
 
 Lemma t2_good__wk :
     exists Δ,
-        (Δ : nil ⊢ t2_good).
+        ( nil ,, Δ : nil ⊢ t2_good # (Kind_Arrow KB KB)).
 Proof with eauto with noDup_db.
     exists (
             (
-             ("X", (Ty_App (Ty_Lam "Y" KB (Ty_App (Ty_Var "Y") (Ty_Var "X"))) (Ty_Lam "Z" KB (Ty_Var "X"))))
+             ("X", (Ty_App (Ty_Lam "Y" (Kind_Arrow (Kind_Arrow KB KB) (Kind_Arrow KB KB)) (Ty_App (Ty_Var "Y") (Ty_Var "X"))) (Ty_Lam "Z" (Kind_Arrow KB KB) (Ty_Var "X"))))
             ::([("Y", (Ty_App (Ty_Var "Y") (Ty_Var "X")))]
             ++ ("Z", (Ty_Var "X"))::nil))
             ++
             [("V", (Ty_Var "V"))])%list.
     unfold t2_good.
-    apply ND_App.
+    apply ND_App with (K1 := (Kind_Arrow KB KB)).
     - apply ND_Lam.
-      apply ND_App.
-      apply ND_Lam.
-      rewrite empty_concat.
-      constructor.
-      constructor. apply in_eq. constructor. apply in_cons. apply in_eq.
       
-      unfold P_ND2'. intros. inversion H.
-      unfold P_Dup_Normal. intros. inversion H.
-      unfold P_BF. intros. intros Hcontra. simpl in Hcontra. assumption.
-      unfold P_BF. intros. inversion H. subst. simpl. intuition. congruence. inversion H0.
+      eapply ND_App.
       apply ND_Lam.
-      constructor. apply in_cons. apply in_eq.
-      unfold P_BF. intros. inversion H. subst. simpl. intuition. congruence. inversion H0.
-      unfold P_ND2'. intros. inversion H0. inversion H1. subst.
-      inversion H. inversion H2. subst. inversion H2. inversion H1.
-      unfold P_Dup_Normal. intros. subst. inversion H0. inversion H1. subst.
-      inversion H. inversion H2. inversion H2. inversion H1.
-      unfold P_BF. intros. inversion H. subst. intros Hcontra.
-      simpl in Hcontra.
-      inversion Hcontra.
-      congruence.
-      inversion H0.
-      congruence.
-      exact H1.
-      inversion H0.
-      unfold P_BF. intros. inversion H.
+      assert ([("Y",
+      Kind_Arrow (Kind_Arrow KB KB)
+        (Kind_Arrow KB KB));
+      ("X", Kind_Arrow KB KB)],,
+      ([] ++ []) : ["Y"; "X"]
+      ⊢ (Ty_App (Ty_Var "Y")
+        (Ty_Var "X"))
+      # Kind_Arrow KB KB).
+      {
+        econstructor.
+        econstructor. apply in_eq. constructor. 
+        + simpl. constructor. apply in_cons. apply in_eq. simpl.
+          auto.
+        + 
+        
+        unfold P_ND2'. intros. inversion H.
+        +
+          unfold P_Dup_Normal. intros. inversion H.
+        + unfold P_BF. intros. intros Hcontra. simpl in Hcontra. assumption.
+      }
+      { rewrite <- empty_concat in H. assumption. }
+      { unfold P_BF. intros. inversion H. subst. simpl. intuition. congruence. inversion H0. }
+      { apply ND_Lam.
+        constructor. apply in_cons. apply in_eq. simpl. auto.
+        unfold P_BF. intros. inversion H. subst. simpl. intuition. congruence. inversion H0. }
+        unfold P_ND2'. intros. inversion H0. inversion H1. subst.
+        inversion H. inversion H2. subst. inversion H2. inversion H1.
+        unfold P_Dup_Normal. intros. subst. inversion H0. inversion H1. subst.
+        inversion H. inversion H2. inversion H2. inversion H1.
+        unfold P_BF. intros. inversion H. subst. intros Hcontra.
+        simpl in Hcontra.
+        inversion Hcontra.
+        congruence.
+        inversion H0.
+        congruence.
+        exact H1.
+        inversion H0.
+        unfold P_BF. intros. inversion H.
     - apply ND_Lam.
       constructor. apply in_eq.
+      simpl. auto. 
       unfold P_BF. intros. inversion H.
     - unfold P_ND2'. intros.
       inversion H0.
@@ -360,21 +406,16 @@ Proof.
     reflexivity.
 Qed.
 
+Definition x0_double := Ty_Lam "X" KB (Ty_Lam "X" KB (Ty_Var "X")).
 
-(** Kinding of types *)
-Reserved Notation "Δ '|-*' T ':' K" (at level 40, T at level 0, K at level 0).
-Inductive has_kind : list (string * kind) -> ty -> kind -> Prop :=
-  | K_Var : forall Δ X K,
-      lookup X Δ = Some K ->
-      Δ |-* (Ty_Var X) : K
-  | K_Lam : forall Δ X K1 T K2,
-      ((X, K1) :: Δ) |-* T : K2 ->
-      Δ |-* (Ty_Lam X K1 T) : (Kind_Arrow K1 K2)
-  | K_App : forall Δ T1 T2 K1 K2,
-      Δ |-* T1 : (Kind_Arrow K1 K2) ->
-      (drop_btv Δ (btv T1)) |-* T2 : K1 -> (* This rule makes that a well-kinded type can never have capture when evaluated one step*)
-      Δ |-* (Ty_App T1 T2) : K2
-where "Δ '|-*' T ':' K" := (has_kind Δ T K).
+Lemma x0_double_wk :
+        ([] ,, [("X", (KB, (Ty_Lam "X" KB (Ty_Var "X"))));("X", (KB, (Ty_Var "X")))] : [] ⊢ x0_double # (Kind_Arrow KB (Kind_Arrow KB KB))).
+Proof.
+  constructor.
+  repeat constructor.
+  unfold P_BF. intros. inversion H. subst. simpl. intuition.
+  (* NO, not ok, which is good! *)
+Admitted.
 
 Theorem well_kinded__no_capture :
     (* Maybe:
@@ -419,35 +460,35 @@ Fixpoint duplicate {A : Type} (l : list A) (n : nat ) :=
   end.
 
 (* collect binders*)
-Fixpoint dsubst' (T : ty) : list (string * ty) :=
+Fixpoint dsubst' (T : ty) : list (string * (kind * ty)) :=
   match T with
   | Ty_Var X => []
   | Ty_Lam Y K T_body =>
-    (Y, T_body)::(dsubst' T_body)
+    (Y, (K, T_body))::(dsubst' T_body)
   | Ty_App T1 T2 =>
     dsubst' T1 ++ dsubst' T2
   end.
 
 (* This is the property that we want to prove: that the step relation preserves the typing property *)
 
-Fixpoint dsubst (Δ2 : list (string * ty)) (X : string) (U : ty) (T : ty): list (string * ty) :=
+Fixpoint dsubst (Δ2 : list (string * (kind * ty))) (X : string) (U : ty) (T : ty): list (string * (kind * ty)) :=
   match T with
   | Ty_Var Y => if X =? Y then Δ2 else nil
   | Ty_App T1 T2 => 
       (dsubst Δ2 X U T1 ++ dsubst Δ2 X U T2)%list
   | Ty_Lam Y K T_body =>
     if X =? Y then
-      (Y, T_body)::(dsubst' T_body)
+      (Y, (K, T_body))::(dsubst' T_body)
     else 
-      (Y, substituteT X U T_body)::(dsubst Δ2 X U T_body)
+      (Y, (K, substituteT X U T_body))::(dsubst Δ2 X U T_body)
   end.
 
 Lemma BF_propertyΔ :
-    forall (Δ : list (string * ty)) (Γ : list string) (T : ty) (X : string),
-        Δ : Γ ⊢ T ->
+    forall Ξ (Δ : list (string * (kind * ty))) (Γ : list string) (T : ty) K (X : string),
+        Ξ ,, Δ : Γ ⊢ T # K ->
         In X Γ -> ~ In X (map fst Δ).
 Proof.
-  intros Δ Γ T X Hnd.
+  intros Ξ Δ Γ T K X Hnd.
   generalize dependent X.
   induction Hnd; intros.
   - auto.
@@ -463,39 +504,512 @@ Proof.
     apply not_in_app. split; eauto.
 Qed.
 
+Inductive SubTy : ty -> ty -> Prop :=
+  | ST_Var : forall X,
+      SubTy (Ty_Var X) (Ty_Var X)
+  | ST_Lam : forall X K T1 T2,
+      SubTy T1 T2 ->
+      SubTy (Ty_Lam X K T1) (Ty_Lam X K T2)
+  | ST_Lam2 : forall X Y K K2 T1 T2,
+      SubTy (Ty_Lam X K T1) T2 ->
+      SubTy (Ty_Lam X K T1) (Ty_Lam Y K2 T2)
+  | ST_App : forall T1 T1' T2 T2',
+      SubTy T2 T2' ->
+      SubTy T1 T1' ->
+      SubTy (Ty_App T1 T2) (Ty_App T1' T2')
+  | ST_AppL : forall T1 T1' T2,
+      SubTy T1 T1' ->
+      SubTy T1 (Ty_App T1' T2)
+  | ST_AppR : forall T1 T2 T2',
+      SubTy T2 T2' ->
+      SubTy T2 (Ty_App T1 T2').
+
+
+Lemma subTy_refl T :
+  SubTy T T.
+Proof.
+  induction T; simpl; constructor; auto.
+Qed.
+
+(* IF T1 is a subtype of T2, then it cannot have bigger kind
+  WRONG IT CAN:
+  Take T1 = x, with X in context * -> *
+  Then T = x T2 for T2 : *, will have kind *.
+*)
+Lemma subTy_of_normal__smaller_kind Ξ Δ1 Δ2 Γ1 Γ2 T1 T2 K1 K2:
+    Ξ ,, Δ1 : Γ1 ⊢ T1 # K1 ->
+    Ξ ,, Δ2 : Γ2 ⊢ T2 # K2 ->
+    SubTy T1 T2 -> normal_Ty T2 -> kind_size K1 <= kind_size K2.
+Proof.
+  intros Hwk1 Hwk2 Hsub Hnorm.
+  generalize dependent Ξ.
+  generalize dependent Δ1.
+  generalize dependent Δ2.
+  generalize dependent Γ1.
+  generalize dependent Γ2.
+  generalize dependent K1.
+  generalize dependent K2.
+  induction Hsub; intros.
+  - inversion Hwk1; subst.
+    inversion Hwk2; subst.
+    assert (K1 = K2).
+    {
+      rewrite H6 in H4.
+      inversion H4.
+      auto.
+    }
+    subst.
+    lia.
+  - inversion Hwk1; subst.
+    inversion Hwk2; subst.
+    simpl.
+    assert (kind_size K3 <= kind_size K0).
+    {
+      eapply IHHsub; eauto.
+      inversion Hnorm; subst; auto.
+      inversion H.
+    }
+    lia.
+  - inversion Hwk1; subst.
+    inversion Hwk2; subst.
+    admit.
+  - (* T1' T2' is normal, then the whole thing is neutral
+      what do we know about kind_size of neutral things? probably the sum
+    *)
+  
+    inversion Hwk1; subst.
+    inversion Hwk2; subst.
+    assert (kind_size K0 <= kind_size K3).
+    {
+      eapply IHHsub1; eauto.
+      inversion Hnorm; subst; auto.
+      inversion H. subst.
+      assumption.
+    }
+    assert (kind_size (Kind_Arrow K0 K1) <= kind_size (Kind_Arrow K3 K2)).
+    {
+      eapply IHHsub2; eauto.
+      inversion Hnorm; subst; auto.
+      inversion H0; subst.
+      apply NO_neutral in H11. assumption.
+    }
+    simpl in H0.
+    (* kind_size K1, is the kind_size of the application*)
+    admit.
+  - 
+Admitted.
+
+Lemma kind_size_not_zero K :
+  kind_size K > 0.
+Proof.
+  induction K; simpl; auto.
+  lia.
+Qed.
+
+Lemma btv_implies_Δ {Ξ Δ Γ T K X} :
+  Ξ ,, Δ : Γ ⊢ T # K -> 
+  In X (btv T) -> 
+  In X (map fst Δ).
+Proof.
+Admitted.
+
+Lemma Δ_implies_subTy Ξ Δ Γ T K X T' K' :
+  Ξ ,, Δ : Γ ⊢ T # K -> 
+  In (X, (K', T')) Δ -> 
+  SubTy (Ty_Lam X K' T') T.
+Proof.
+  intros Hwk Hin.
+  generalize dependent T'.
+  generalize dependent K'.
+  induction Hwk; subst; intros.
+  - inversion Hin.
+  - inversion Hin.
+    + inversion H0; subst.
+      apply subTy_refl.
+    + specialize (IHHwk K' T' H0).
+      apply ST_Lam2.
+      assumption.
+  - apply in_app_or in Hin.
+    destruct Hin as [Hin1 | Hin2].
+    + apply ST_AppL.
+      eapply IHHwk1; eauto.
+    + apply ST_AppR.
+      eapply IHHwk2; eauto.
+Qed.
+
+
+Lemma wk_norm_P2 X T Δ Δ2 KU Ξ Γ K U :
+  P_ND2' ((X, (KU, T))::Δ) Δ2 ->
+  Ξ ,, ((X, (KU, T))::Δ) : Γ ⊢ Ty_Lam X KU T # Kind_Arrow KU K ->
+  Ξ ,, Δ2 : Γ ⊢ U # KU ->
+  normal_Ty U ->
+  ~ In X (map fst Δ2).
+Proof.
+  assert (kind_size KU < kind_size (Kind_Arrow KU K)).
+  {
+    simpl.
+    remember (kind_size KU) as n.
+    assert (kind_size K > 0).
+    {
+      apply kind_size_not_zero.
+    }
+    lia.
+  }
+  intros.
+  intros Hcontra.
+  assert (kind_size (Kind_Arrow KU K) <= kind_size KU).
+  {
+    eapply subTy_of_normal__smaller_kind; eauto.
+    assert (In (X, (KU, T)) Δ2).
+    {
+      
+      unfold P_ND2' in H0.
+      apply in_map_iff in Hcontra as [[X' [K' T']] [Hfst Hsnd]].
+      inversion Hfst. simpl in H4. subst. simpl.
+      assert ((KU, T) = (K', T')).
+      {
+        eapply H0; eauto.
+        simpl.
+        left. auto.
+      }
+      inversion H5.
+      subst.
+      assumption.
+    }
+    eapply Δ_implies_subTy; eauto.
+  }
+  lia.
+Qed.
+
+(* Some property about duplicates and normality*)
+Lemma wk_norm_P X T Δ Δ2 KU Ξ Γ K U :
+  ~ In X Γ ->
+  P_ND2' ((X, (KU, T))::Δ) Δ2 ->
+  ((X, KU)::Ξ) ,, Δ : (X :: Γ) ⊢ T # K ->
+  Ξ ,, Δ2 : Γ ⊢ U # KU ->
+  normal_Ty U ->
+  ~ In X (map fst Δ2).
+Proof.
+  (* My intuitioin: Then λ X KU T is a SubTy of U, and that cannot be well-kinded,  *)
+  intros.
+  intros.
+  eapply wk_norm_P2; eauto.
+  constructor.
+  eauto.
+  unfold P_BF.
+  intros.
+  simpl.
+  intuition.
+  subst.
+  intuition.
+  eapply BF_propertyΔ in H1.
+  eauto. apply in_cons. auto.
+Qed.
+
+Lemma P_ND2'_app Δ1 Δ1' Δ2 :
+  P_ND2' (Δ1 ++ Δ1')%list Δ2 ->
+  P_ND2' Δ1 Δ2 /\ P_ND2' Δ1' Δ2.
+Proof.
+  intros.
+  split.
+  + unfold P_ND2' in H.
+    unfold P_ND2'.
+    intros.
+    eapply H.
+    apply in_app_iff.
+    left. auto. eauto. auto.
+  + unfold P_ND2' in H.
+    unfold P_ND2'.
+    intros.
+    eapply H.
+    apply in_app_iff.
+    right. auto. eauto. auto.
+Qed.
+
+Lemma P_ND2'_cons X K T Δ1 Δ2 :
+  P_ND2' ((X, (K, T))::Δ1) Δ2 ->
+  P_ND2' Δ1 Δ2.
+Proof.
+  intros.
+  unfold P_ND2' in H.
+  unfold P_ND2'.
+  intros.
+  eapply H.
+  apply in_cons. eauto. auto.
+Qed.
+
+Lemma P_Dup_Normal_app Δ1 Δ1' Δ2 :
+  P_Dup_Normal (Δ1 ++ Δ1')%list Δ2 ->
+  P_Dup_Normal Δ1 Δ2 /\ P_Dup_Normal Δ1' Δ2.
+Admitted.
+
+Lemma P_Dup_Normal_cons X K T Δ1 Δ2 :
+  P_Dup_Normal ((X, (K, T))::Δ1) Δ2 ->
+  P_Dup_Normal Δ1 Δ2.
+Admitted.
+
+Lemma P_BF_App Δ1 Δ2 Γ :
+  P_BF (Δ1 ++ Δ2) Γ <->
+  P_BF Δ1 Γ /\ P_BF Δ2 Γ.
+Admitted.
+
+Lemma dsubst_split Δ2 X X0 U T :
+  In X (map fst (dsubst Δ2 X0 U T)) -> (In X (map fst Δ2) \/ In X (btv T)).
+Proof.
+Admitted.
+
+Lemma dsubst_split2 Δ2 X X0 U T T':
+  In (X, T') ( (dsubst Δ2 X0 U T)) -> (In (X, T') (Δ2) \/ In (X, T') (dsubst' T)).
+Proof.
+Admitted.
+
+(* In other words: λx. λx. y   is not allowed! because same binder name binds different bodies*)
+Lemma P_ND2'_refl Ξ ΔU Γ U KU :
+  Ξ ,, ΔU : Γ ⊢ U # KU ->
+  P_ND2' ΔU ΔU.
+Proof.
+  intros Hwk.
+  unfold P_ND2'.
+  intros.
+  generalize dependent KT.
+  generalize dependent KT'.
+  generalize dependent X.
+  induction Hwk; intros.
+  - inversion H1.
+  - destr_eqb_eq X X0.
+    + subst.
+      apply BF_propertyΔ with (X := X0) in Hwk; eauto.
+      * inversion H0.
+        -- inversion H2; subst.
+           inversion H1; subst.
+            inversion H3; subst. auto.
+            eapply in_map with (f := fst) in H3.
+            simpl in H3.
+            contradiction.
+        -- inversion H0; inversion H1.
+            inversion H3; subst. inversion H4; subst. auto.
+            eapply in_map with (f := fst) in H2.
+            contradiction.
+            eapply in_map with (f := fst) in H3.
+            contradiction.
+            eapply in_map with (f := fst) in H4.
+            contradiction.
+
+      * apply in_eq.
+    + inversion H0.
+      * inversion H3. contradiction.
+      * inversion H1. inversion H4. contradiction.
+        eapply IHHwk; eauto.
+  - apply in_app_or in H2 as [H2 | H2].
+    + eapply IHHwk1; eauto.
+      apply in_app_or in H3 as [H3 | H3].
+      auto. 
+      unfold P_ND2' in H.
+      specialize (H X KT' KT H2 H3).
+      subst.
+      auto.
+    + eapply IHHwk2; eauto.
+      apply in_app_or in H3 as [H3 | H3].
+      auto.
+      unfold P_ND2' in H.
+      specialize (H X KT KT' H3 H2).
+      subst.
+      auto. auto.
+Qed.
+
+Lemma P_Dup_Normal_refl Ξ ΔU Γ U KU :
+  Ξ ,, ΔU : Γ ⊢ U # KU ->
+  normal_Ty U ->
+  P_Dup_Normal ΔU ΔU.
+Proof.
+  intros.
+  unfold P_Dup_Normal.
+  intros.
+  inversion H3; subst; clear H3.
+  generalize dependent T'.
+  generalize dependent K2.
+  generalize dependent X.
+  induction H; intros.
+  - inversion H2.
+  - inversion H2; subst.
+    + inversion H4; subst.
+      inversion H0; subst.
+      assumption.
+      inversion H5.
+    + eapply IHWK; eauto.
+      inversion H0; subst; auto.
+      inversion H5.
+  - apply in_app_or in H5 as [H5 | H5].
+    + eapply IHWK1; eauto.
+      inversion H0; subst; auto.
+      inversion H7; subst.
+      apply NO_neutral in H10.
+      assumption.
+    + eapply IHWK2; eauto.
+      inversion H0; subst; auto.
+      inversion H7; subst.
+      apply NO_neutral in H10.
+      assumption.
+Qed.
+
+    
+
+Lemma P_ND2'_dsubst Ξ KU Γ Δ1 Δ2 ΔU X U T1 T2 K1 K2:
+  Ξ ,, ΔU : Γ ⊢ U # KU ->
+  ((X, KU)::Ξ) ,, Δ1 : (X:: Γ) ⊢ T1 # K1 ->
+  ((X, KU)::Ξ) ,, Δ2 : (X :: Γ ) ⊢ T2 # K2 ->
+  P_ND2' Δ1 Δ2 ->
+  P_ND2' ΔU Δ1 ->
+  P_ND2' ΔU Δ2 ->
+  P_Dup_Normal Δ1 Δ2 ->
+  normal_Ty U ->
+  (P_ND2' (dsubst ΔU X U T1) (dsubst ΔU X U T2) /\ 
+    P_Dup_Normal (dsubst ΔU X U T1) (dsubst ΔU X U T2)).
+Proof.
+  intros Hwk_U Hwk_T1 Hwk_T2 HPND2'_T HPDN_T Hnorm_U.
+  assert (HP_ND2'_ΔU: P_ND2' ΔU ΔU).
+  {
+    eapply P_ND2'_refl; eauto.
+  }
+  split.
+  - unfold P_ND2'.
+    intros X0 KT KT' HIn_dT1 HIn_dT2.
+    (* Suppose (X0, KT) is in dsubst ΔU X U T1,
+      Then it is originally a lambda in T1, or in ΔU,
+        or it is a binder in substituteT X U T1
+
+        What if T1 = λ (Y.Y).
+
+        And T2 = X (λY.Y)
+
+        Then dsubst ΔU X U T1 = [(Y, Y)]
+
+        dsubst ΔU X U T2 = ΔU ++ [Y, Y].
+        Now, this is only problematic if there is then some binder Y in ΔU, that maps to something else
+          than Y. But that is not allowed by P_ND2' ΔU Δ2.
+
+        Hmm. But do we have some sort of no_dup of binders?
+    *)
+
+    admit.
+  - 
+      
+      
+        (* Unsure*) admit.
+Admitted.
+
+(* When stepping, we never introduce new binders (no capture-avoiding stuff)*)
+Lemma P_BF_step Δ1 Δ1' Ξ Γ T1 T1' K :
+  P_BF Δ1 Γ ->
+  Ξ ,, Δ1 : Γ ⊢ T1 # K ->
+  Ξ ,, Δ1' : Γ ⊢ T1' # K ->
+  step T1 T1' ->
+  P_BF Δ1' Γ.
+Admitted.
+
+Lemma P_ND2'_step Δ1 Δ2 Δ2' Ξ Γ T2 T2' K2 K2' :
+  P_ND2' Δ1 Δ2 ->
+  P_Dup_Normal Δ1 Δ2 ->
+  step T2 T2' ->
+  Ξ ,, Δ2 : Γ ⊢ T2 # K2 ->
+  Ξ ,, Δ2' : Γ ⊢ T2' # K2' ->
+  (P_ND2' Δ1 Δ2' /\ P_Dup_Normal Δ1 Δ2').
+Proof.
+  intros PND_Δ2 PDupN_Δ2 Hstep Hwk_T2 Hwk_T2'.
+  split.
+  - unfold P_ND2'.
+    intros X KT KT' HIn_Δ1 HIn_Δ2'.
+    (* If X, KT in Δ2' and Δ1, then (X, KT) in Δ2*)
+    (* If (X, KT') in Δ2' then there must be a key X in Δ2
+    *)
+    assert (In (X, KT) Δ2).
+    {
+      (* By P_ND2' Δ1 Δ2, then it must be (X, KT), and by P_Dup_Normal, KT is normal*)
+      admit.
+    }
+    assert (normal_Ty (snd KT)) by admit.
+    (* By P_ND2'_Dup, we know that all X-lambdas in Δ2 are normal and equal.
+      Δ2 corresponds to T2, so all X-lambdas in T2 are normal and equal
+
+      Step T2 T2'
+
+      This step cannot have occured inside of one of these lambdas, because they are normal
+      It could have beta reduced?
+
+      T2 = (λV. (λX. f(V)))) (P!)
+
+      Then only problematic if also (λX. V) in Δ1.
+      But that is not possible, then v free in T1.
+       What if it is bound in T1?
+       Then it must be the same as in T2, and that is not possible, because not normal...
+
+       hmmmmm subtle....
+      Suppose (λX. f(V)) changed. then there must have been an variable in there.
+      call it V.
+      Then V must have been bound in T2, otherwise it would not have been substituted.
+      
+      We only have a problem if also (λX. f(V)) in Δ1.
+      V can either be free or bound in T1.
+      - V free in T1:
+        Then V free in T1, and bound in T2. But by
+          Ξ,, Δ : Γ ⊢ (Ty_App T1 T2) # K
+        We have BF Δ Γ. And then V in fst Δ, and V in Γ. contradiction.
+      - V bound in T1. i.e. (λV. ... f(V))
+        Then because V also bound in T2, and P_ND2' Δ1 Δ2, we must have
+           (V, (K, λX. f(V))) in Δ2. But fuck. That is fine.
+
+      Hmm. But with real beta reduction with our step function, this situation can never happen
+      We only start substituting (and hence doubling, once nothign can be substituted 
+      in this term anymore (a λv surround it can not exist: it cannot have been in Δ1
+      by BF).
+
+    )
+    *)
+
+
+
+    admit.
+Admitted.
+
 (* This is the property that we want to prove: that the step relation preserves the typing property *)
 
 (* HMM, I do not seem to use this for open U? *)
-Theorem substituteT_preserves_NoDup : forall T Δ1 Δ2 Γ X U,
-  P_ND2' ((X, T)::Δ1) Δ2 ->
-  P_Dup_Normal ((X, T)::Δ1) Δ2 ->
-  (* P_BF (((X, T)::Δ1) ++ Δ2) Γ -> *)  (* Hopefully we do not need this *)
+Theorem substituteT_preserves_NoDup : forall Ξ T Δ1 Δ2 Γ X U KU K,
+  P_ND2' (Δ1) Δ2 ->
+  P_Dup_Normal (Δ1) Δ2 ->
   normal_Ty U ->
-  Δ1 : (X :: Γ) ⊢ T ->
-  Δ2 : Γ ⊢ U -> (* This lemma is used where X was in a lambda binder: hence, by the new typing rule, it may not occur free in U*)
-  dsubst Δ2 X U T : Γ ⊢ (substituteT X U T).
+  ((X, KU)::Ξ) ,, Δ1 : (X :: Γ) ⊢ T # K  ->
+  Ξ ,, Δ2 : Γ ⊢ U # KU -> (* This lemma is used where X was in a lambda binder: hence, by the new typing rule, it may not occur free in U*)
+  P_BF (((X, (KU, T))::nil)) Γ ->  (* Hopefully we do not need this *)
+  Ξ ,, (dsubst Δ2 X U T) : Γ ⊢ (substituteT X U T) # K.
 Proof with eauto.
     
-    intros T Δ1 Δ2 Γ X U HPND2 HDupNo HNo HndT HndU.
+    intros Ξ T Δ1 Δ2 Γ X U KU K HPND2 HDupNo HNo HndT HndU HBF.
     generalize dependent Δ2.
     generalize dependent Δ1.
     generalize dependent Γ.
     generalize dependent U.
+    generalize dependent Ξ.
+    generalize dependent K.
+    generalize dependent KU.
+    generalize dependent X.
     
-    induction T.
+    induction T; intros.
     - (* Var *)
-      intros.
       simpl.
       destr_eqb_eq X s.
       + inversion HndT; subst.
         unfold dsubst. auto.
+        simpl in H4. rewrite String.eqb_refl in H4. inversion H4. subst. assumption.
       + inversion HndT; subst.
         constructor.
-        inversion HndT.
-        subst.
-        inversion H3; subst.
-        congruence.
-        auto.
+        * simpl in H1.
+          destruct H1; auto.
+          contradiction.
+        * simpl in H5.
+          rewrite <- String.eqb_neq in H.
+          rewrite H in H5.
+          assumption.
     - (* Lam *)
       intros.
       
@@ -504,170 +1018,154 @@ Proof with eauto.
       + (* X = s*)
         exfalso.
         inversion HndT; subst.
-        unfold P_BF in H5.
-        specialize (H5 s).
-        contradiction H5.
+        unfold P_BF in H7.
+        specialize (H7 s).
+        contradiction H7.
         apply in_eq. simpl. left. reflexivity.
       + (* X <> s *)
         inversion HndT; subst.
         
-        assert (WK_Dup' Δ (X :: s :: Γ) T).
+        assert (WK ((X, KU)::(s, k)::Ξ) Δ (X :: s :: Γ) T K2).
         {
             (* ADMIT: Weakening: cons_permute *)
             admit.
         }
         apply ND_Lam.
-        eapply IHT; eauto.
-        * (* ADMIT:
-        TODO: This is the trickest case.
-          U normal.   U can be of the form .... (λ(s: K). T) ...
-          Then it must have kind >= kind of (λ (s : K). T), since this must be inside of
-          a lambda body. it cannot be in head position by normality.
-        
-             What if X in Δ2? If it appears in there, it must have the exact same form:
-            (X, Ty_Lam s k T), but that cannot be well-kinded... the argument must have smaller kind
-
-            We cannot hide it in a const function or something: it is normal.
-          *)
-          admit.
-        * (* ADMIT: By above, X cannot occur in Δ2, hence this hold trivially by above*)
-           admit.
-        * (* ADMIT: Weakening Gamma *) admit.
-        * (* hmm, new case.
-        
-            
-          *)
-          unfold P_BF.
-          intros.
-          simpl.
-          intuition.
-          -- subst.
-             unfold P_BF in H6.
-             specialize (H6 X0).
-             contradiction H6.
-             apply in_cons. auto. simpl. left. reflexivity.
-          -- (* By P_BF we know X0 not in the binders of T (i.e. Δ)
-              What about Δ2?
-              Can only happen if X free in T.
-              
-              So we would need: P_BF Δ2 Γ
-            *)
-            apply BF_propertyΔ with (X := X0) in HndU.
-            (* Then we know X0 notin map fst Δ2!*)
+        {
+          eapply IHT; eauto.
+          * unfold P_BF.
+            intros.
+            inversion H1.
+            subst. simpl. intuition. simpl. intuition. 
+            subst.
+            unfold P_BF in HBF.
+            simpl in HBF.
+            specialize (HBF X0 H2).
+            intuition.
+          
+          * eapply P_ND2'_cons; eauto.
+          * eapply P_Dup_Normal_cons; eauto.
+          * (* ADMIT: Weakening Gamma *) 
+            (* 
+              What if s is already in Ξ? 
+              By P_BF we know s not free in Gamma.
+              Then s not free in U.
+              Then s not necessary in Ξ, then we might shadow, but it is not important.
+              *)
             admit.
-            auto.
+          
+            
+          
+        }
+        unfold P_BF.
+        intros.
+        simpl.
+        intuition.
+        -- subst.
+          unfold P_BF in H8.
+          specialize (H8 X0).
+          contradiction H8.
+          apply in_cons. auto. simpl. left. reflexivity.
+        -- apply BF_propertyΔ with (X := X0) in HndU; eauto.
+           assert (In X0 (map fst Δ2) \/ In X0 (btv T)).
+           {
+            eapply dsubst_split; eauto.
+           }
+           destruct H2 as [H2 | H2].
+           ++ contradiction.
+           ++ assert (In X0 (map fst Δ)).
+              {
+                eapply btv_implies_Δ; eauto.
+              }
+              unfold P_BF in H8.
+              specialize (H8 X0).
+              assert (In X0 (X :: Γ)).
+              {
+                simpl. intuition.
+              }
+              specialize (H8 H5).
+              simpl in H8.
+              intuition.
+            
+
     - intros.
       simpl.
       inversion HndT; subst.
-      assert (dsubst Δ2 X U (Ty_App T1 T2) = (dsubst Δ2 X U T1 ++ dsubst Δ2 X U T2)%list).
-      {
-        simpl. reflexivity.
-      }
-      constructor; eauto.
+      
+      econstructor; eauto.
       + eapply IHT1; eauto.
-        * (* ADMIT:
-            By P_ND2', if X in Δ2, then it is in there with (X, Ty_App T1 T2).
-               That cannot be, that must be ill-kinded, since it is normal?
-
-            Tricky tricky tricky (see also lam case):
-            App case. Kind of U is smaller than kind of T1. So then how can the whole of 
-              Ty_App T1 T2 be in U? It must then be normal (T1 neutral). Hence in whatever
-              term, by normality, its kind will occur in the final kind: it cannot be 
-              removed with some smart function or something, this is vague.
-
-          *)
-           admit.
-        * (* See above, X cannot be in there.*)
-          admit.
+        * eapply P_ND2'_app in HPND2 as [HPND2 _].
+          assumption.
+        * eapply P_Dup_Normal_app in HDupNo as [HDupNo _].
+          assumption.
       + eapply IHT2; eauto.
-        * (* ADMIT: see above *) admit.
-        * (* ADMIT: see above *) admit.
-      + (* Everything in Δ2 must for sure be normal, it will be in both sides.
-            I think that it is by normality of U.
-          Suppose (X, T) is a type in Δ0.
-
-          If also (X, T') in Δ3, then T = T'.
-          Then we substitute in identical terms, should be no problem.
-
-          If X not in Δ3, but X in Δ2? By:
-            P_Dup_Normal Δ0 Δ2
-            and P_Dup_Normal Δ3 Δ2
-          *)
-      
-      
-        (* Unsure*) admit.
-      + (* See above *)
-
-        (* Unsure *) admit.
-      + (*
-          P_BF will decompose over app.
-          Then dsubst will never have more binders than Δ0, Δ2, Δ3, U, added,
-          and they all have no binders that are free in Γ by assumption.
-            (Suppose U has a binder, then that binder is also in Δ2.)
-        *)
-      
-        (* Unsure *) admit.
-
+        * eapply P_ND2'_app in HPND2 as [_ HPND2].
+          assumption.
+        * eapply P_Dup_Normal_app in HDupNo as [_ HDupNo].
+          assumption.
+      + eapply P_ND2'_dsubst with (Ξ := Ξ) (Δ1 := Δ0) (Δ2 := Δ3); eauto.
+        * eapply P_ND2'_app in HPND2 as [HPND2 _].
+          apply P_ND2'_sym.
+          assumption.
+        * eapply P_ND2'_app in HPND2 as [_ HPND2].
+          apply P_ND2'_sym.
+          assumption.
+      + eapply P_ND2'_dsubst with (Δ1 := Δ0) (Δ2 := Δ3); eauto.
+        * eapply P_ND2'_app in HPND2 as [HPND2 _].
+          apply P_ND2'_sym.
+          assumption.
+        * eapply P_ND2'_app in HPND2 as [_ HPND2].
+          apply P_ND2'_sym.
+          assumption.
+      + apply P_BF_App.
+        apply P_BF_App in H9 as [P_BFΔ0 P_BFΔ3].
+        split.
+        * unfold P_BF.
+          intros.
+          intros Hcontra.
+          apply dsubst_split in Hcontra.
+          destruct Hcontra as [Hcontra | Hcontra].
+          -- eapply BF_propertyΔ in HndU; eauto.
+          -- apply (btv_implies_Δ H1) in Hcontra.
+             eapply BF_propertyΔ in H1; eauto.
+             apply in_cons. assumption.
+        * unfold P_BF.
+          intros.
+          intros Hcontra.
+          apply dsubst_split in Hcontra.
+          destruct Hcontra as [Hcontra | Hcontra].
+          -- eapply BF_propertyΔ in HndU; eauto.
+          -- apply (btv_implies_Δ H2) in Hcontra.
+             eapply BF_propertyΔ in H2; eauto.
+             apply in_cons. assumption.
 Admitted.
 
 (* This is the property that we want to prove: that the step relation preserves the typing property *)
-Theorem preservation' T1 T2 Δ Γ :
-    Δ : Γ ⊢ T1 -> step T1 T2 -> exists Δ', Δ' : Γ ⊢ T2.
+Theorem preservation' Ξ T1 T2 Δ Γ K :
+    Ξ ,, Δ : Γ ⊢ T1 # K -> step T1 T2 -> exists Δ', Ξ ,, Δ' : Γ ⊢ T2 # K.
 Proof.
     intros Hnd Hstep.
     generalize dependent Δ.
     generalize dependent Γ.
+    generalize dependent K.
+    generalize dependent Ξ.
     induction Hstep; intros.
     - inversion Hnd; subst; clear Hnd.
       inversion H1; subst; clear H1.
 
-      (* What do we know:
-        T is WF under Δ2.
-        T normal.
-        Δ : (X :: Γ) ⊢ S,  so X free in S.
-        We know, if X in Δ2, then S is normal.
-        So why would this hold?
-        Ftvs are not changed by substituteT, so let's ignore Gamma?
-
-        From
-          Δ : (X :: Γ) ⊢ S
-
-          we should conclude
-
-          f(Δ) : Γ ⊢ substituteT X T S
-
-        I think maybe we know that (X, S)::Δ contains no duplicates.
-          I think that follows from Δ : (X :: Γ) ⊢ S, the BF property.
-        
-        Let's say S = λY. (λZ. Y X) (λV. X)
-        Then Δ = (Y, (λZ. Y X) (λV. X)) :: (Z, Y X) :: (V, X) :: nil)).
-        
-        This term would become (substituteT X T S) = (λY. (λZ. Y T) (λV. T)),
-        but T the binders of T (say T = λW. W) should be carefully included into Δ.
-
-        If T = λW. W, then substituteT X T S =
-          (λY. (λZ. Y (λW. W)) (λV. (λW. W)))
-        Which must have
-          (Y, (λZ. Y (λW. W)) (λV. (λW. W))) :: (Z, Y (λ W. W))
-            :: (W, W)
-            :: (V, (λ W. W))
-            :: (W, W)
-           :: nil)).
-          
-        Maybe we can find some algorithm for that?
-        We traverse Δ, whenever we see X, replace with T.
-        Whenever in this entry X is not surrounded by a lambda anymore,
-        add new entries Δ2
-
-        So it is a function f(Δ, Δ2, X, T) that returns Δ'.
-
-        But why would we have the properties?
-
-
-      *)
-      assert (dsubst Δ2 X T S : Γ ⊢ (substituteT X T S)).
+      assert (Ξ ,, (dsubst Δ2 X T S) : Γ ⊢ (substituteT X T S) # K0).
       {
-        eapply substituteT_preserves_NoDup; eauto.
+        eapply substituteT_preserves_NoDup with (Δ1 := Δ); eauto.
+        + eapply P_ND2'_cons; eauto.
+        + eapply P_Dup_Normal_cons; eauto.
+        + unfold P_BF.
+          intros. simpl.
+          intuition.
+          subst.
+          unfold P_BF in H13.
+          specialize (H13 X0 H).
+          simpl in H13.
+          intuition.
       }
       exists (dsubst Δ2 X T S)%list.
       assumption.
@@ -675,65 +1173,55 @@ Proof.
     - (* Analogous to below *)
       admit.
     - inversion Hnd; subst.
-      specialize (IHHstep Γ Δ2 H2) as [Δ2' Hnd2'].
+      specialize (IHHstep Ξ K1 Γ Δ2 H2) as [Δ2' Hnd2'].
       exists (Δ1 ++ Δ2')%list.
-      constructor; auto.
-      + (* Something, say (X, T) in Δ2' stepped. so we could have lost this property if 
-            X is a key in Δ1. 
-            But by P_Dup_Normal, we know that then it could not have stepped (by normality).
-        *)
-        admit.
-      + (* P_DUP ? *)
-        admit.
-      + (* Δ2' is obtained from Δ2 by stepping. Hence bvs Δ2' are subset of bvs Δ2, so no problem*)
-        admit.
+      apply ND_App with (K1 := K1); auto.
+      + eapply P_ND2'_step with (Δ2 := Δ2) (K2' := K1) (K2 := K1); eauto.
+      + eapply P_ND2'_step with (Δ2 := Δ2) (K2' := K1) (K2 := K1); eauto.
+      + apply P_BF_App in H9 as [H9 H10].
+        apply P_BF_App; split; auto.
+        eapply P_BF_step; eauto.
     - inversion Hnd; subst.
-      specialize (IHHstep (bX :: Γ) Δ0 H2) as [Δ0' Hnd0'].
-      exists ((bX, T2)::Δ0')%list.
+      specialize (IHHstep ((bX, K)::Ξ) K2 (bX :: Γ) Δ0 H6) as [Δ0' Hnd0'].
+      exists ((bX, (K, T2))::Δ0')%list.
       constructor; auto.
-Admitted.
-
-(* Even after stepping, the type is still typeable in the more restrictive TyApp rule
-  meaning that even after stepping, when stepping again, we will again not have capture
-  i.e. this is the property that GU implies that is preserved
-  under normalisation/betaReduction.
-*)
-Theorem preservation T1 T2 Δ K :
-    Δ |-* T1 : K -> step T1 T2 -> Δ |-* T2 : K.
-Proof.
-    intros Hwk Hstep.
-    generalize dependent Δ.
-    generalize dependent K.
-    induction Hstep; intros.
-    - inversion Hwk; subst.
-      inversion H2; subst.
-      assert ((drop_btv Δ (btv S)) |-* T : K1).
-      {
-        (* Weakening, we coulud potentially add X, but it cannot be free in T by H4*)
-        admit.
-      }
-      eapply substituteT_preserves_kinding; eauto.
-    - inversion Hwk; subst.
-      apply K_App with (K1 := K1).
-      + eapply IHHstep; eauto.
-      + (* stepping does not introduce new btvs, 
-        but it could remove them, hence
-            btv S2  subset of  btv S1
-
-            Hence 
-               inclusion (drop_btv Δ (btv s1)) (drop_btv Δ (btv s2))
-            reasoning: btv s1 is bigger than btv s2: we remove more, hence lookup in the first implies still lookup in the second, which has every element in the first, and possibly more
-
-            But what about shadowing??? I fear the existence of an X that becomes visible, but then that X was not necessary to begin with. So no issue.
-
-        *)
-        admit.
-    - inversion Hwk; subst.
-      apply K_App with (K1 := K1).
-      + assumption.
-      + eapply IHHstep; eauto.
-    - inversion Hwk; subst.
-      constructor.
-      eapply IHHstep; eauto.
-      
+      inversion Hnd0'; subst.
+      + unfold P_BF. intros. unfold P_BF in H7.
+        specialize (H7 X0 H1).
+        simpl.
+        simpl in H7.
+        intuition.
+      + unfold P_BF. intros.
+        simpl. intuition.
+        -- subst.
+            unfold P_BF in H7.
+            specialize (H7 X0 H1).
+            simpl in H7.
+            intuition.
+         -- subst.
+            unfold P_BF in H0.
+            specialize (H0 X0).
+            assert (In X0 (bX :: Γ)).
+            {
+              simpl. intuition.
+            }
+            specialize (H0 H2).
+            simpl in H0.
+            intuition.
+         -- unfold P_BF in H0.
+            contradiction H0 with (X := X0).
+            apply in_cons. assumption.
+            simpl. right. auto.
+      + unfold P_BF.
+        intros.
+        simpl.
+        intuition; subst.
+        eapply BF_propertyΔ in Hnd; eauto.
+        simpl in Hnd. intuition.
+        rewrite map_app in H8.
+        apply in_app_or in H8 as [H8 | H8].
+        * eapply BF_propertyΔ in H; eauto.
+          apply in_cons. assumption.
+        * eapply BF_propertyΔ in H0; eauto.
+          apply in_cons. assumption.
 Admitted.
